go/iterator/traceIter.go
@@ -1,0 +1,21 @@
+package iterator
+
+func isAscii(str []byte) bool {
+	ret_val := true
+
+	var loop_body func(int) bool = func (i int) bool {
+		if (str[i] >= 0x80 || str[i] == 0x00) {
+			ret_val = false
+			return false
+		}
+
+		ret_val = true
+		return true
+	}
+
+	iterator := intIter(len(str))
+
+	iterator(loop_body)
+
+	return ret_val
+}
